## Note
nid: 1619941750310
model: Basic-d7a3e-4ce08
tags: 02_vorlesung
markdown: false

### Front
Explain how the Sum of Squares Total can be decomposed into <b>Sum
of Squares Regression (SSR)</b> and the <b>Sum of Squared Errors
(SSE)</b>.

### Back
\[\text{SST} = \text{SSR} + \text{SSE}\]
<div>
  where:
</div>
<div>
  \[\begin{array}{c} S S
  R=\sum_{i=1}^{n}\left(\hat{y}_{i}-\bar{y}\right)^{2} \\ S S
  E=\sum_{i=1}^{n}\left(y_{i}-\hat{y}_{i}\right)^{2}=\sum_{i=1}^{n}
  e_{i}^{2} \end{array}\]
</div>
<div>
  where \(\hat{y}\) is the estimated value for \(y\) from the
  regression.
</div>
